You are an expert solver of challenging math problems.

---

Let $q > 1$ be a power of $2$. Let

$$f : \mathbb{F}*{q^2} \to \mathbb{F}*{q^2}$$

be an affine map over $\mathbb{F}_2$. Show that the equation

$$f(x) = x^{q+1}$$

has at most $2q - 1$ solutions.

Here, $\mathbb{F}*{q^2}$ denotes the Galois Field (or finite field) of order $q^2$.

---

Let \(q=2^{m}>1\), \(K=\mathbb F_q\subset F=\mathbb F_{q^{2}}\), and let
\[
\operatorname{Tr}(x)=x+x^{q}\in K,\qquad \operatorname{N}(x)=x^{q+1}\in K
\]
be the relative trace and norm \(F\to K\).

Because \(f\) is affine over \(\mathbb F_{2}\), there is an \(\mathbb F_{2}\)-linear map \(L:F\to F\) and a constant \(c\in F\) such that
\[
f(x)=L(x)+c,\qquad\text{and in particular }L(x+y)=L(x)+L(y),\ L(0)=0.
\]
(So \(c=f(0)\).)

Let
\[
S=\{x\in F:\ f(x)=x^{q+1}\}
\]
be the solution set. We will show \(|S|\le 2q-1\).

---

## 1) A key computation: translating by elements of \(K\)

Fix \(x\in F\) and \(a\in K\). Since \(a^{q}=a\), we have
\[
(x+a)^{q+1}=(x+a)(x^{q}+a)=xx^{q}+a(x+x^{q})+a^{2}.
\]
Equivalently,
\[
(x+a)^{q+1}=x^{q+1}+a\,\operatorname{Tr}(x)+a^{2}. \tag{1}
\]

Also, since \(f(x)=L(x)+c\) and \(L\) is additive,
\[
f(x+a)=L(x+a)+c=L(x)+L(a)+c=f(x)+L(a). \tag{2}
\]

Now suppose \(x\in S\), i.e. \(f(x)=x^{q+1}\). Put \(t=\operatorname{Tr}(x)\in K\). Then \(x+a\) is also a solution iff
\[
f(x+a)=(x+a)^{q+1}.
\]
Using (1) and (2) and canceling \(f(x)=x^{q+1}\), this becomes
\[
L(a)=a^{2}+t\,a. \tag{3}
\]

So for a **fixed** trace value \(t\in K\), the allowed translations \(a\in K\) that preserve solutions are exactly those satisfying (3).

This motivates the definition:

\[
A_t:=\{a\in K:\ L(a)=a^{2}+t\,a\}\subseteq K. \tag{4}
\]

(Notice \(0\in A_t\) for every \(t\), since \(L(0)=0\).)

---

## 2) Solutions with the same trace form one coset of \(A_t\)

For each \(t\in K\), define the “trace slice”
\[
S_t:=\{x\in S:\ \operatorname{Tr}(x)=t\}.
\]
Then \(S\) is the disjoint union of the \(S_t\), so
\[
|S|=\sum_{t\in K}|S_t|. \tag{5}
\]

### Claim.
For each \(t\in K\), either \(S_t=\varnothing\), or else \(S_t\) is a translate (coset) of \(A_t\), hence \(|S_t|=|A_t|\).

**Proof.**

- If \(S_t=\varnothing\), done.

- Otherwise pick one solution \(x_0\in S_t\) with \(\operatorname{Tr}(x_0)=t\).
  We show \(S_t=x_0+A_t\).

  First, if \(a\in A_t\), then (3) holds with \(x=x_0\), so \(x_0+a\in S\). Also \(\operatorname{Tr}(a)=a+a^q=a+a=0\) (since \(a\in K\) and \(\mathrm{char}=2\)), hence
  \(\operatorname{Tr}(x_0+a)=\operatorname{Tr}(x_0)=t\). Thus \(x_0+A_t\subseteq S_t\).

  Conversely, take any \(x\in S_t\). Then \(\operatorname{Tr}(x)=\operatorname{Tr}(x_0)\), so
  \[
  \operatorname{Tr}(x-x_0)=0.
  \]
  In a quadratic extension \(F/K\), \(\operatorname{Tr}(u)=0\) is equivalent to \(u\in K\) (because \(\operatorname{Tr}(u)=u+u^q=0 \iff u^q=u\iff u\in K\)).
  Hence \(a:=x-x_0\in K\). Since both \(x_0\) and \(x_0+a=x\) are solutions with trace \(t\), condition (3) forces \(a\in A_t\). Thus \(x\in x_0+A_t\), proving \(S_t\subseteq x_0+A_t\).

Therefore \(S_t=x_0+A_t\), so \(|S_t|=|A_t|\). ∎

From (5) and the claim we immediately get the useful inequality
\[
|S|=\sum_{t\in K}|S_t|\le \sum_{t\in K}|A_t|. \tag{6}
\]

So it remains to bound \(\sum_{t\in K}|A_t|\).

---

## 3) Counting \(\sum_{t\in K}|A_t|\)

Fix \(a\in K\). For which \(t\in K\) does \(a\in A_t\) hold?

By definition (4),
\[
a\in A_t \iff L(a)=a^2+t\,a.
\]

- If \(a=0\), this is true for every \(t\) (both sides \(=0\)). So \(a=0\) contributes \(q\) to the total sum \(\sum_t |A_t|\).

- If \(a\ne 0\), then rearranging gives
  \[
  t=\frac{L(a)+a^2}{a}. \tag{7}
  \]
  This determines **at most one** \(t\) (uniquely) once \(a\) is fixed.

  However, \(t\) must lie in \(K\). Since \(a\in K^*\) and \(a^2\in K\), the right-hand side is in \(K\) **iff** \(L(a)\in K\). (Dividing by \(a\in K^*\) does not change membership in \(K\).)

  So:
  - if \(L(a)\notin K\), then \(a\) belongs to **no** \(A_t\);
  - if \(L(a)\in K\), then \(a\) belongs to **exactly one** \(A_t\).

Therefore, among nonzero \(a\in K^*\), each contributes either \(0\) or \(1\) to \(\sum_t |A_t|\). Hence
\[
\sum_{t\in K}|A_t|
= q \;+\; \bigl|\{a\in K^*:\ L(a)\in K\}\bigr|
\le q + (q-1)
=2q-1. \tag{8}
\]

---

## 4) Finish

Combining (6) and (8),
\[
|S|\le \sum_{t\in K}|A_t|\le 2q-1.
\]

So the equation
\[
f(x)=x^{q+1}
\]
has at most \(2q-1\) solutions in \(\mathbb F_{q^2}\), as required. ∎

---

### Where the hypothesis “\(q\) is a power of \(2\)” is used
It is used crucially in the translation formulas:
- \(\operatorname{Tr}(a)=a+a^q=0\) for \(a\in K\) relies on characteristic \(2\) (so \(a+a=0\)),
- and \((x+a)^{q+1}=x^{q+1}+a\operatorname{Tr}(x)+a^2\) simplifies nicely because \(a^q=a\) and cross terms behave additively in characteristic \(2\).

If you want, I can also show an example where equality \(2q-1\) is attained (for suitable choices of \(f\)).